Add the last 4 blocks of padding to the Tar data. Change the way tar header filenames are found. Make sure tar header returns a Fetch. Subset (Disk) proofs for Tar stuff

Tar.v
@@ -31,26 +31,6 @@ Fixpoint fromOctalAscii (bytes: list Byte) : Exc N :=
     end
   end.
 
-Definition diskIsFound (disk: Disk) (nextVal: N) :=
-  match (disk nextVal) with
-  | Found _ => true
-  | _ => false
-  end.
-
-Lemma diskIsFound_subset:
-  forall (sub super: Disk) (offset val: N),
-    sub ⊆ super ->
-      diskIsFound sub offset = true ->
-        diskIsFound super offset = true.
-Proof.
-  intros sub super offset val subset.
-  unfold diskIsFound. intros H.
-  destruct (sub offset) eqn:found.
-    apply subset in found. rewrite found. reflexivity.
-    discriminate H.
-    discriminate H.
-Qed.
-
 Definition parseFileName (tar: File) (offset: N) (disk: Disk): @Fetch string :=
   N.peano_rect
   (fun _ => N -> @Fetch string) (* Signature of recursive calls *)
@@ -78,75 +58,79 @@ Lemma parseFileName_subset:
         parseFileName tar offset super = Found val.
 Proof.
   unfold parseFileName.
+  generalize 0.
   apply N.peano_ind with (n := 100).
     simpl; auto.
-  intros n H sub super tar offset val subset H1.
+  intros n H m sub super tar offset val subset H1.
   rewrite N.peano_rect_succ.
   rewrite N.peano_rect_succ in H1.
-  destruct (tar @[ offset + 0 | sub ]) eqn:TarAt.
+  destruct (tar @[ offset + m | sub ]) eqn:TarAt;
+      [| discriminate H1 | discriminate H1].
   apply fetchByte_subset with (1:=subset) in TarAt.
   rewrite TarAt. 
-  rewrite <- H1. simpl.
-  (*
-  destruct (ascii_eqb b zero). assumption.
-  simpl in H1. simpl.
-  rewrite <- H1. discriminate.
-  apply H in H1.
+  destruct (ascii_eqb b zero) eqn:IsZero.
   assumption.
-
-  apply N.recursion_succ.
-  destruct val.
-  apply N.peano_rect_base.
-  apply N.peano_ind with (n := 100).
-    intros sub super tar offset val subset.
-    simpl; auto.
-  intros sub super tar offset.
-  revert sub 
-  intros sub super tar offset str subset.
-  revert sub super 
-  unfold parseFileName.
-  apply N.peano_ind with (n := 100).
-  simpl. auto.
-  intros. rewrite N.peano_rect_succ.
-  assert (exists v:Byte, tar @[ offset + 0 | sub ] = Found v).
-  admit.
-  destruct H1.
-  apply fetchByte_subset with (1:=subset) in H1.
-  rewrite H1. simpl.
-  destruct (ascii_eqb x zero).
-  remember (tar @[ offset + 0 | sub]).
-  destruct f.
-    eauto.
-  simpl in H0.
-
-  remember (tar @[offset + 0 | 
-  simpl.
-  destruct (tar @[ offset + 0 | super]).
-  apply
+  match goal with   (* match helps us reference subterms in the goal *)
+    | [ _: match ?peano with _ => _ end = _ |- _] => 
+        destruct peano eqn:Hpeano; [| discriminate H1 | discriminate H1]
+  end.
+  apply H with (1:=subset) in Hpeano. rewrite Hpeano. 
+  assumption.
 Qed.
-*)
-Admitted.
 
 
-Definition parseFileSize (bytes: ByteData) :=
-  (seq_list bytes 124 11)
-    _fflatmap_ (fun fileSizeList =>
-    match (fromOctalAscii fileSizeList) with
-    | error => ErrorString "Invalid Tar Size"
+Definition parseFileSize (tar: File) (offset: N) (disk: Disk): @Fetch N :=
+  (tar @[ offset + 124 | disk ]) _fflatmap_ (fun byte0 =>
+  (tar @[ offset + 125 | disk ]) _fflatmap_ (fun byte1 =>
+  (tar @[ offset + 126 | disk ]) _fflatmap_ (fun byte2 =>
+  (tar @[ offset + 127 | disk ]) _fflatmap_ (fun byte3 =>
+  (tar @[ offset + 128 | disk ]) _fflatmap_ (fun byte4 =>
+  (tar @[ offset + 129 | disk ]) _fflatmap_ (fun byte5 =>
+  (tar @[ offset + 130 | disk ]) _fflatmap_ (fun byte6 =>
+  (tar @[ offset + 131 | disk ]) _fflatmap_ (fun byte7 =>
+  (tar @[ offset + 132 | disk ]) _fflatmap_ (fun byte8 =>
+  (tar @[ offset + 133 | disk ]) _fflatmap_ (fun byte9 =>
+  (tar @[ offset + 134 | disk ]) _fflatmap_ (fun byte10 =>
+    match (fromOctalAscii (byte0 :: byte1 :: byte2 :: byte3
+                           :: byte4 :: byte5 :: byte6 :: byte7
+                           :: byte8 :: byte9 :: byte10 :: nil)) with
+    | error => 
+        if ((Byte.eqb byte0 Ascii.zero) && (Byte.eqb byte1 Ascii.zero)
+            && (Byte.eqb byte2 Ascii.zero) && (Byte.eqb byte3 Ascii.zero)
+            && (Byte.eqb byte4 Ascii.zero) && (Byte.eqb byte5 Ascii.zero)
+            && (Byte.eqb byte6 Ascii.zero) && (Byte.eqb byte7 Ascii.zero)
+            && (Byte.eqb byte8 Ascii.zero) && (Byte.eqb byte9 Ascii.zero)
+            && (Byte.eqb byte10 Ascii.zero))
+          (* the last few chunks of the Tar file are full of zeros *)
+          then Found 0
+          (* something went wrong *)
+          else ErrorString "Invalid Tar Size"
     | value size => Found size
-    end).
+    end))))))))))).
+
+Lemma parseFileSize_subset:
+  forall (sub super: Disk) (tar: File) (offset: N) (val: N),
+    sub ⊆ super ->
+      parseFileSize tar offset sub = Found val ->
+        parseFileSize tar offset super = Found val.
+Proof.
+  intros sub super tar offset val subset.
+  unfold parseFileSize.
+  unfold disk_subset in subset.
+  repeat (apply found_fflatmap_found_twice; [
+    intros ?; apply fetchByte_subset with (1:=subset)
+    | intro; intro]).
+  intros. assumption.
+Qed.
+
 
 Definition parseFileNameAndSize (tar: File) (offset: N) 
-  (disk: Disk)
-  : @Fetch (string*N) :=
-  let byteData := shift (fetchByte tar.(fileId) disk) 
-                        offset in
+  (disk: Disk) : @Fetch (string*N) :=
   (parseFileName tar offset disk) _fflatmap_ (fun name =>
-  (parseFileSize byteData) _fmap_ (fun size =>
+  (parseFileSize tar offset disk) _fmap_ (fun size =>
     (name, size)
   )).
 
-(*
 Lemma parseFileNameAndSize_subset:
   forall (sub super: Disk) (tar: File) (offset: N) (val: string*N),
     sub ⊆ super ->
@@ -158,18 +142,20 @@ Proof.
   intros H.
   apply found_fflatmap_found in H. destruct H as [fileName [HfileName H]].
   apply found_fmap_found in H. destruct H as [size [Hsize H]].
-  rewrite fetchByte_subset in HfileName.
-*)
+  apply parseFileName_subset with (1:=subset) in HfileName.
+  rewrite HfileName. unfold fetch_flatmap at 1.
+  apply parseFileSize_subset with (1:=subset) in Hsize.
+  rewrite Hsize. unfold fetch_map at 1.
+  rewrite H. auto.
+Qed.
 
 
-Definition recFileNameFrom (nextCall: N -> list string) 
-  (tar: File) (remaining: N) (disk: Disk) : list string :=
-  if (remaining <=? 0)
-    then nil
+Definition recFileNameFrom (nextCall: N -> @Fetch (list string))
+  (tar: File) (offset: N) (disk: Disk) : @Fetch (list string) :=
+  if (tar.(fileSize) <=? offset)
+    then Found nil
   else match 
-    (parseFileNameAndSize tar
-                          (tar.(fileSize) - remaining) 
-                          disk) with
+    (parseFileNameAndSize tar offset disk) with
     | Found (fileName, fileSize) =>
         (* Strip the next file out of the tar *)
         (* Round to the nearest 512 *)
@@ -177,37 +163,89 @@ Definition recFileNameFrom (nextCall: N -> list string)
           if (fileSize mod 512 =? 0)
           then fileSize + 512
           else 512 * (2 + (fileSize / 512))) in
-        fileName :: (nextCall (remaining - nextFileSize))
-    | _ => nil
+        match (nextCall (offset + nextFileSize)) with
+        | Found rest => Found (fileName :: rest)
+        | MissingAt val => MissingAt val
+        | ErrorString val => ErrorString val
+        end
+    | MissingAt val => MissingAt val
+    | ErrorString val => ErrorString val
     end.
 
-Definition parseFileNames (file: File) (disk: Disk): list string :=
+Definition parseFileNames (file: File) (disk: Disk): @Fetch (list string) :=
   N.peano_rect
-  (fun _ => N -> list string) (* Signature of recursive calls *)
-  (fun (_: N) => nil:(list string)) (* Base case -- empty file *)
-  (fun (prev: N) (rec: N -> list string) (remaining: N) =>
+  (fun _ => N -> @Fetch (list string)) (* Signature of recursive calls *)
+  (fun (_: N) => Found (nil:(list string))) (* Base case -- empty file *)
+  (fun (prev: N) (rec: N -> @Fetch (list string)) (offset: N) =>
     (* Recursive case -- more file remaining *)
-    recFileNameFrom rec file remaining disk)  
+    recFileNameFrom rec file offset disk)  
   file.(fileSize)
-  file.(fileSize).
+  0.
+
+Lemma parseFileNames_subset:
+  forall (sub super: Disk) (file: File) (val: list string),
+    sub ⊆ super ->
+      parseFileNames file sub = Found val ->
+        parseFileNames file super = Found val.
+Proof.
+  unfold parseFileNames. 
+  intros sub super file. revert sub super.
+  generalize 0.
+  apply N.peano_ind with (n := fileSize file).
+    simpl; auto.
+  intros n H m sub super val subset H1.
+  rewrite N.peano_rect_succ.
+  rewrite N.peano_rect_succ in H1.
+  unfold recFileNameFrom at 1.
+  unfold recFileNameFrom at 1 in H1.
+  destruct (fileSize file <=? m) eqn:H_fileSize.
+    assumption.
+  destruct (parseFileNameAndSize file m sub) eqn:H_fileNameAndSize;
+    [| discriminate H1 | discriminate H1].
+  destruct p as [fileName fileSize]. 
+  apply parseFileNameAndSize_subset with (1:=subset) in H_fileNameAndSize.
+  rewrite H_fileNameAndSize.
+  destruct (fileSize mod 512 =? 0) eqn:H_fsize_mod_512.
+  simpl. simpl in H1.
+  match goal with   (* match helps us reference subterms in the goal *)
+    | [ _: match ?peano with _ => _ end = _ |- _] => 
+        destruct peano eqn:Hpeano; [| discriminate H1 | discriminate H1]
+  end.
+  apply H with (1:=subset) in Hpeano. rewrite Hpeano.
+  assumption.
+  cbv zeta. cbv zeta in H1.
+  destruct (N.peano_rect (fun _ : N => N -> Fetch) (fun _ : N => Found nil)
+                         (fun (_ : N) (rec : N -> Fetch) (offset : N) =>
+                         recFileNameFrom rec file offset sub) n
+                         (m + 512 * (2 + fileSize / 512))) eqn:Hpeano;
+    [|discriminate H1 | discriminate H1].
+  apply H with (1:=subset) in Hpeano. rewrite Hpeano.
+  assumption.
+Qed.
 
 Definition looksLikeRootkit (file: File) (disk: Disk) :=
-  let fileNames := parseFileNames file disk in
-  exists (filename1 filename2: string),
-    filename1 <> filename2
-    /\ In filename1 fileNames
-    /\ In filename2 fileNames
-    /\ (FileNames.systemFile filename1)
-    /\ (FileNames.systemFile filename2).
+  match (parseFileNames file disk) with
+  | Found fileNames =>
+    exists (filename1 filename2: string),
+      filename1 <> filename2
+      /\ In filename1 fileNames
+      /\ In filename2 fileNames
+      /\ (FileNames.systemFile filename1)
+      /\ (FileNames.systemFile filename2)
+  | _ => False
+  end.
 
 Definition looksLikeRootkit_compute (file: File) (disk: Disk)
   (filename1 filename2: string) :=
-  let fileNames := parseFileNames file disk in
-     (negb (string_eqb filename1 filename2))
-  && (existsb (string_eqb filename1) fileNames)
-  && (existsb (string_eqb filename2) fileNames)
-  && (FileNames.systemFile_compute filename1)
-  && (FileNames.systemFile_compute filename2).
+  match (parseFileNames file disk) with
+  | Found fileNames =>
+       (negb (string_eqb filename1 filename2))
+    && (existsb (string_eqb filename1) fileNames)
+    && (existsb (string_eqb filename2) fileNames)
+    && (FileNames.systemFile_compute filename1)
+    && (FileNames.systemFile_compute filename2)
+  | _ => false
+  end.
 
 Lemma looksLikeRootkit_reflection (file: File) (disk: Disk)
   (filename1 filename2: string) :
@@ -216,6 +254,7 @@ Lemma looksLikeRootkit_reflection (file: File) (disk: Disk)
 Proof.
   intros. unfold looksLikeRootkit_compute in H. 
   unfold looksLikeRootkit.
+  destruct (parseFileNames file disk); [|discriminate H | discriminate].
   apply Bool.andb_true_iff in H. destruct H.
   apply Bool.andb_true_iff in H. destruct H.
   apply Bool.andb_true_iff in H. destruct H.
@@ -234,4 +273,20 @@ Proof.
     apply systemFile_reflection. auto.
 
     apply systemFile_reflection. auto.
+Qed.
+
+Lemma looksLikeRootkit_subset:
+  forall (sub super: Disk) (file: File),
+    sub ⊆ super ->
+      looksLikeRootkit file sub ->
+        looksLikeRootkit file super.
+Proof.
+  intros sub super file subset.
+  unfold looksLikeRootkit.
+  intros H.
+  destruct (parseFileNames file sub) eqn:H_parseFileNames.
+    apply parseFileNames_subset with (1:=subset) in H_parseFileNames.
+    rewrite H_parseFileNames. assumption.
+  contradict H.
+  contradict H.
 Qed.
